prove Scalars.store_sep; use in swap

bedrock2/src/Examples/swap.v
@@ -3,13 +3,12 @@ Require Import bedrock2.BasicC64Syntax bedrock2.NotationsInConstr.
 Import Syntax BinInt String List.ListNotations.
 Local Open Scope string_scope. Local Open Scope Z_scope. Local Open Scope list_scope.
 Local Existing Instance bedrock2.BasicC64Syntax.StringNames_params.
-Local Coercion literal (z : Z) : Syntax.expr := Syntax.expr.literal z.
 Local Coercion var (x : string) : Syntax.expr := Syntax.expr.var x.
 
 Definition swap := ("swap", (["a";"b"], ([]:list varname), bedrock_func_body:(
-  "t" = *(uint8_t*) "b";;
-  *(uint8_t*) "b" = *(uint8_t*) "a";;
-  *(uint8_t*) "a" = "t"
+  "t" = *(uintptr_t*) "b";;
+  *(uintptr_t*) "b" = *(uintptr_t*) "a";;
+  *(uintptr_t*) "a" = "t"
 ))).
 
 Definition swap_swap := ("swap_swap", (("a"::"b"::nil), ([]:list varname), bedrock_func_body:(
@@ -21,62 +20,27 @@ Require bedrock2.WeakestPrecondition.
 Require Import bedrock2.Semantics bedrock2.BasicC64Semantics.
 Require Import coqutil.Map.Interface bedrock2.Map.Separation bedrock2.Map.SeparationLogic.
 
-Local Instance FIXME_mem_ok : map.ok Semantics.mem.
-Admitted. (* FIXME *)
-
+Axiom __map_ok : map.ok Semantics.mem. Local Existing Instance __map_ok. (* FIXME *)
 
 Require bedrock2.WeakestPreconditionProperties.
-From coqutil.Tactics Require Import eabstract.
-Require Import bedrock2.ProgramLogic.
+From coqutil.Tactics Require Import letexists eabstract.
+Require Import bedrock2.ProgramLogic bedrock2.Scalars.
 
 Local Infix "*" := sep.
 Local Infix "*" := sep : type_scope.
 Instance spec_of_swap : spec_of "swap" := fun functions =>
   forall a_addr a b_addr b m R t,
-    (ptsto a_addr a * (ptsto b_addr b * R)) m ->
+    (scalar access_size.word a_addr a * (scalar access_size.word b_addr b * R)) m ->
     WeakestPrecondition.call (fun _ => True) (fun _ => False) (fun _ _ => True) functions
       "swap" t m [a_addr; b_addr]
-      (fun t' m' rets => t=t'/\ (ptsto a_addr b * (ptsto b_addr a * R)) m' /\ rets = nil).
+      (fun t' m' rets => t=t'/\ (scalar access_size.word a_addr b * (scalar access_size.word b_addr a * R)) m' /\ rets = nil).
 
 Instance spec_of_swap_swap : spec_of "swap_swap" := fun functions =>
   forall a_addr a b_addr b m R t,
-    (ptsto a_addr a * (ptsto b_addr b * R)) m ->
+    (scalar access_size.word a_addr a * (scalar access_size.word b_addr b * R)) m ->
     WeakestPrecondition.call (fun _ => True) (fun _ => False) (fun _ _ => True) functions
       "swap_swap" t m [a_addr; b_addr]
-      (fun t' m' rets => t=t' /\ (ptsto a_addr a * (ptsto b_addr b * R)) m' /\ rets = nil).
-
-From coqutil.Tactics Require Import eabstract letexists syntactic_unify.
-Require Import coqutil.Datatypes.PrimitivePair.
-Import coqutil.Word.Interface.
-
-Lemma load1_sep a (v:Semantics.byte) R m (H:(ptsto a v * R) m) :
-  load Syntax.access_size.one m a = Some (word.of_Z (LittleEndian.combine 1 (pair.mk v tt))).
-  cbv [load load_bytes bytes_per footprint
-       HList.tuple.map HList.tuple.option_all HList.tuple.unfoldn
-       map.getmany_of_tuple].
-  eapply get_sep in H. rewrite H.
-  exact eq_refl.
-Qed.
-
-Lemma store1_sep a (v1:Semantics.byte) v2 (R:mem->Prop) (m:mem) (H : sep (ptsto a v1) R m)
-    (p := (ptsto a (pair._1 (LittleEndian.split 1 (word.unsigned v2)))))
-    (post : mem -> Prop) (cont : forall (m':mem), sep p R m' -> post m') :
-  exists (m':mem), store Syntax.access_size.one m a v2 = Some m' /\ post m'.
-Proof.
-Admitted.
-
-Lemma split_combine_1 a :
-  (pair._1 (LittleEndian.split 1 (word.unsigned (word.of_Z (LittleEndian.combine 1 (pair.mk a tt )))))) = a.
-Proof.
-  cbn -[word.of_Z word.unsigned].
-  rewrite Z.lor_0_r.
-Admitted.
-
-Ltac sep :=
-  let m := lazymatch goal with |- _ ?m => m end in
-  let H := multimatch goal with H: _ m |- _ => H end  in
-  refine (Lift1Prop.subrelation_iff1_impl1 _ _ _ _ _ H); clear H;
-  SeparationLogic.ecancel; fail.
+      (fun t' m' rets => t=t' /\ (scalar access_size.word a_addr a * (scalar access_size.word b_addr b * R)) m' /\ rets = nil).
 
 Lemma swap_ok : program_logic_goal_for_function! swap.
 Proof.
@@ -85,27 +49,15 @@ Proof.
   letexists. split. exact eq_refl. (* argument initialization *)
 
   repeat straightline.
-  letexists; split.
-  { repeat straightline. letexists; split; [eapply load1_sep; sep|repeat straightline]. }
-
+  eapply Scalars.store_sep; [solve[SeparationLogic.ecancel_assumption]|].
   repeat straightline.
-  letexists; split.
-  { repeat straightline. letexists; split; [eapply load1_sep; sep|repeat straightline]. }
-
+  eapply Scalars.store_sep; [solve[SeparationLogic.ecancel_assumption]|].
   repeat straightline.
-  eapply store1_sep; [sep|].
 
-  repeat straightline.
-  eapply store1_sep; [sep|].
-
-  repeat straightline.
   (* final postcondition *)
   split. exact eq_refl.
   split. 2:exact eq_refl.
-  repeat match goal with x := _ |- _ => subst x end.
-  rewrite word.unsigned_of_Z in H0.
-  rewrite 2split_combine_1 in *.
-  assumption.
+  SeparationLogic.ecancel_assumption.
 Defined.
 
 Lemma swap_swap_ok : program_logic_goal_for_function! swap_swap.
@@ -115,24 +67,23 @@ Proof.
   letexists. split. exact eq_refl. (* argument initialization *)
 
   repeat straightline.
-  straightline_call; [sep|].
+  straightline_call; [solve[SeparationLogic.ecancel_assumption]|].
   repeat straightline.
   letexists; split.
   { exact eq_refl. }
 
   repeat straightline.
-  straightline_call; [sep|].
+  straightline_call; [solve[SeparationLogic.ecancel_assumption]|].
   repeat straightline.
   letexists; split.
   { exact eq_refl. }
 
   repeat straightline.
-
   repeat split; assumption.
 Defined.
 
 Lemma link_swap_swap_swap_swap : spec_of_swap_swap (swap_swap::swap::nil).
 Proof. auto using swap_swap_ok, swap_ok. Qed.
 
-(* Print Assumptions link_swap_swap_swap_swap. *)
-(* store1_sep SortedList.sorted_remove SortedList.sorted_put SortedList.map_ok fst_split0_combine0 *)
+Print Assumptions link_swap_swap_swap_swap.
+(* __map_ok SortedListString.string_strict_order SortedList.sorted_remove SortedList.sorted_put StrictOrderWord *)
